Nearly all done

verif_tuplekey/verif_inthash.v
@@ -1,8 +1,15 @@
+Require Import VST.progs.conclib.
 Require Import VST.floyd.proofauto.
 Require Import inthash.
 Require FMapWeakList.
 Require Import Program.Basics. Open Scope program_scope.
 Require Import Structures.OrdersEx.
+
+Definition N: Z := 10.
+Global Opaque N.
+Lemma N_eq: N = 10. reflexivity. Qed.
+Hint Rewrite N_eq: rep_omega.
+
 Instance CompSpecs : compspecs. make_compspecs prog. Defined.
 Definition Vprog : varspecs. mk_varspecs prog. Defined.
 
@@ -12,20 +19,20 @@ Require Import VST.floyd.library.
 
 Definition V := sig is_pointer_or_null.
 Definition nullV: V := exist _ nullval mapsto_memory_block.is_pointer_or_null_nullval.
-Definition N: Z := 10.
 
 Module int_table := FMapWeakList.Make Z_as_DT.
-Print int_table.
+
+Notation "{{ m }}" := (int_table.this m).
 
 Section IntTable.
   Import int_table.
   Check SetoidList.InA .
-  Definition get_buckets (m: t V): list (list (Z*V)) :=
-    List.map (fun n => filter (fun kv => eq_dec (fst kv mod N) (Z.of_nat n)) (elements m)) (seq 0%nat (Z.to_nat N)).
+  Definition get_buckets (m: t V): list (int_table.Raw.t V) :=
+    List.map (fun n => filter (fun kv => eq_dec (fst kv mod N) (Z.of_nat n)) {{ m }}) (seq 0%nat (Z.to_nat N)).
 
   Lemma Zlength_get_buckets: forall m, Zlength (get_buckets m) = N.
   Proof.
-    intros []. cbn.
+    intros []. unfold get_buckets. cbn.
     rewrite Zlength_map, Zlength_correct, seq_length. reflexivity.
   Qed.
 
@@ -33,20 +40,20 @@ Section IntTable.
     forall k v, MapsTo k v m <-> SetoidList.InA (eq_key_elt (elt := V)) (k, v) (Znth (k mod N) (get_buckets m)).
   Proof.
     intros.
-    unshelve epose proof (Z_mod_lt k N _). unfold N. computable.
+    unshelve epose proof (Z_mod_lt k N _). rep_omega.
     assert (N = Zlength (seq 0%nat (Z.to_nat N))). rewrite Zlength_correct, seq_length. reflexivity.
     assert (mapsto_iff: MapsTo k v m <-> SetoidList.InA (@eq_key_elt _) (k, v) (elements m)).
     split; [apply elements_1 | apply elements_2].
-    rewrite mapsto_iff.
+    rewrite mapsto_iff. clear mapsto_iff.
     destruct m as [l nodup]. unfold get_buckets.
-    rewrite Znth_map, SetoidList.filter_InA.
-    rewrite <- nth_Znth by omega.
-    rewrite seq_nth by now apply Z2Nat.inj_lt.
-    cbn. rewrite Z2Nat.id by omega.
-    now destruct initial_world.EqDec_Z.
-    intros x y hxy. apply Raw.PX.eqke_eqk in hxy. now rewrite hxy.
+    rewrite Znth_map, SetoidList.filter_InA. 
+    rewrite <- sublist.nth_Znth by omega.
+    rewrite seq_nth.
+    cbn. rewrite Z2Nat.id by omega. 
+    destruct eq_dec. intuition. contradiction. rep_omega.
+    intros x y hxy. apply Raw.PX.eqke_eqk in hxy. rewrite hxy; reflexivity.
     rewrite Zlength_correct, seq_length, Z2Nat.id.
-    apply Z_mod_lt. unfold N; omega. unfold N; omega.
+    apply Z_mod_lt. rep_omega. rep_omega.
   Qed.
 
   Lemma NoDupA_filter: forall (m: t V) (p: Z * V -> bool),
@@ -67,10 +74,10 @@ Section IntTable.
   Lemma NoDupA_bucket: forall k m,
     SetoidList.NoDupA (Raw.PX.eqk (elt:=V)) (Znth (k mod N) (get_buckets m)).
   Proof.
-    intros. destruct m.
+    intros k [].
     unfold get_buckets.
-    unshelve epose proof (Z_mod_lt k N _). unfold N. omega.
-    rewrite Znth_map, <- nth_Znth, seq_nth, Nat.add_0_l, Z2Nat.id. apply NoDupA_filter.
+    unshelve epose proof (Z_mod_lt k N _). rep_omega.
+    rewrite Znth_map, <- sublist.nth_Znth, seq_nth, Nat.add_0_l, Z2Nat.id. apply NoDupA_filter.
     intros x y <-; reflexivity.
     omega. rep_omega.
     rewrite Zlength_correct, seq_length; rep_omega.
@@ -84,21 +91,13 @@ Section IntTable.
     forall k v, MapsTo k v m <-> MapsTo k v (get_bucket k m).
   Proof.
     intros. destruct m as [l nodup].
-    unshelve epose proof (Z_mod_lt k N _). unfold N. omega.
+    unshelve epose proof (Z_mod_lt k N _). rep_omega.
     unfold MapsTo, get_bucket, Raw.PX.MapsTo.
     unfold get_buckets, this.
-    rewrite Znth_map, SetoidList.filter_InA, <- nth_Znth, seq_nth, Nat.add_0_l, Z2Nat.id;
-    fold N; try rewrite Zlength_correct, seq_length; try rep_omega.
+    rewrite Znth_map, SetoidList.filter_InA, <- sublist.nth_Znth, seq_nth, Nat.add_0_l, Z2Nat.id;
+    try rewrite Zlength_correct, seq_length; try rep_omega.
     now destruct eq_dec.
     intros x y hxy%Raw.PX.eqke_eqk. rewrite hxy. reflexivity.
-  Qed.
-
-  Lemma MapsTo_inj: forall (m: t V) k v1 v2,
-      MapsTo k v1 m -> MapsTo k v2 m -> v1 = v2.
-  Proof.
-    intros * h1 h2.
-    apply find_1 in h1. apply find_1 in h2.
-    rewrite h1 in h2. now inv h2.
   Qed.
 
   Lemma find_None: forall m k,
@@ -110,20 +109,48 @@ Section IntTable.
     + case_eq (find (elt := V) k m).
       intros v hfind%find_2. specialize (h v). contradiction.
       easy.
-  Qed.      
+  Qed.
+
+  Corollary find_get_bucket (m: t V):
+    forall k, find k m = find k (get_bucket k m).
+  Proof.
+    intro.
+    case_eq (find (elt := V) k m).
+    + intros v hv%find_2.
+      symmetry. apply find_1. now rewrite <- get_buckets_spec'.
+    + intro hnone.
+      symmetry. rewrite find_None in hnone |- *.
+      intros v hcontr.
+      rewrite <- get_buckets_spec' in hcontr.
+      now apply (hnone v).
+  Qed.
+
+  Lemma MapsTo_inj: forall (m: t V) k v1 v2,
+      MapsTo k v1 m -> MapsTo k v2 m -> v1 = v2.
+  Proof.
+    intros * h1 h2.
+    apply find_1 in h1. apply find_1 in h2.
+    rewrite h1 in h2. now inv h2.
+  Qed.
+    
 
 End IntTable.
 
 Definition t_icell := Tstruct _icell noattr.
 Definition t_inthash := Tstruct _inthash noattr.
 
-Fixpoint icell_rep (l: list (Z*V)) (p: val): mpred :=
+Definition maybe {A: Type} (o: option A) (default: A) :=
+  match o with Some a => a | None => default end.
+
+Definition V_repr: V -> val := @proj1_sig _ _.
+
+Fixpoint icell_rep (l: int_table.Raw.t V) (p: val): mpred :=
   match l with
   | [] => !!(p = nullval) && emp
   | (k, v) :: tl => EX q: val,
                     !! (0 <= k < Int.max_unsigned) &&
                        malloc_token Ews t_icell p *
-                    data_at Ews t_icell (Vint (Int.repr k), (proj1_sig v, q)) p *
+                    data_at Ews t_icell (Vint (Int.repr k), (V_repr v, q)) p *
                     icell_rep tl q
   end.
 
@@ -167,7 +194,7 @@ Definition new_icell_spec: ident * funspec :=
  WITH gv: globals, key: Z, value: V, pnext: val, tl: list (Z*V)
  PRE [ _key OF tuint, _value OF tptr tvoid, _next OF tptr t_icell ] 
    PROP( 0 <= key < Int.max_unsigned )
-   LOCAL(gvars gv; temp _key (Vint (Int.repr key)); temp _value (proj1_sig value); temp _next pnext)
+   LOCAL(gvars gv; temp _key (Vint (Int.repr key)); temp _value (V_repr value); temp _next pnext)
    SEP(icell_rep tl pnext; mem_mgr gv)
  POST [ tptr t_icell ] 
    EX p:val,
@@ -184,30 +211,24 @@ Definition inthash_lookup_spec: ident * funspec :=
    SEP(mem_mgr gv; inthash_rep m pm)
  POST [ tptr tvoid ] 
       PROP() 
-      LOCAL(temp ret_temp (match int_table.find key m with
-             | Some res => proj1_sig res
-             | None => Vnullptr
-          end)) 
+      LOCAL(temp ret_temp (V_repr (maybe (int_table.find key m) nullV))) 
       SEP(mem_mgr gv; inthash_rep m pm).
 
 Definition inthash_insert_list_spec: ident * funspec :=
    DECLARE _inthash_insert_list
- WITH gv: globals, l: list (Z * V), key: Z, ppl: val, pl: val
+ WITH gv: globals, l: int_table.t V, key: Z, ppl: val, pl: val
  PRE [ _r0 OF tptr (tptr t_icell), _key OF tuint ] 
-   PROP(0 <= key < Int.max_unsigned; SetoidList.NoDupA (int_table.Raw.PX.eqk (elt:=V)) l)
+   PROP(0 <= key < Int.max_unsigned)
    LOCAL(gvars gv; temp _r0 ppl; temp _key (Vint (Int.repr key)))
-   SEP(mem_mgr gv; data_at Ews (tptr t_icell) pl ppl; icell_rep l pl)
+   SEP(mem_mgr gv; data_at Ews (tptr t_icell) pl ppl; icell_rep (int_table.this l) pl)
  POST [ tptr t_icell ] 
-   EX p_ret: val, EX r: val, EX tl: list (Z*V),
-            let v := match int_table.Raw.find key l with
-                         | Some v => v
-                         | None => nullV
-                           end in
+   EX p_ret: val, EX r: val, EX tl: int_table.Raw.t V,
+            let v := maybe (int_table.find key l) nullV in 
       PROP( )
       LOCAL(temp ret_temp p_ret) 
       SEP(mem_mgr gv; data_at Ews (tptr t_icell) p_ret r * icell_rep ((key, v) :: tl) p_ret;
           ALL v: V, data_at Ews (tptr t_icell) p_ret r * icell_rep ((key, v) :: tl) p_ret -*
-          EX pl: val, data_at Ews (tptr t_icell) pl ppl * icell_rep (int_table.Raw.add key v l) pl).
+          EX pl: val, data_at Ews (tptr t_icell) pl ppl * icell_rep (int_table.Raw.add key v {{ l }}) pl).
 
 Definition inthash_insert_spec: ident * funspec :=
    DECLARE _inthash_insert
@@ -218,7 +239,7 @@ Definition inthash_insert_spec: ident * funspec :=
    SEP(mem_mgr gv; inthash_rep m pm)
  POST [ tptr tvoid ] 
       PROP( ) 
-      LOCAL(temp ret_temp (match int_table.find key m with Some v => proj1_sig v | None => nullval end)) 
+      LOCAL(temp ret_temp (V_repr (maybe (int_table.find key m) nullV))) 
       SEP(mem_mgr gv; inthash_rep (int_table.add key v m) pm).
 
 Definition Gprog : funspecs :=
@@ -235,7 +256,7 @@ Lemma focus_bucket (m: int_table.t V) (key: Z) (buckets_p: list val)
    iter_sepcon (prod_curry icell_rep) (sublist (i + 1) N l)).
 Proof.
   intros l i.
-  assert (0 <= i < N). { apply Z_mod_lt. unfold N. omega. }
+  assert (0 <= i < N). { apply Z_mod_lt. rep_omega. }
   assert (Zlength l = N).
   { unfold l. rewrite Zlength_correct, combine_length.
     rewrite Min.min_l, <- Zlength_correct. apply Zlength_get_buckets.
@@ -248,7 +269,7 @@ Proof.
   erewrite <- sublist_same at 1.
   erewrite sublist_split at 1. f_equal.
   erewrite sublist_split at 1. erewrite sublist_len_1 at 1.
-  unfold l. rewrite <- nth_Znth, combine_nth, nth_Znth, nth_Znth. reflexivity.
+  unfold l. rewrite <- sublist.nth_Znth, combine_nth, sublist.nth_Znth, sublist.nth_Znth. reflexivity.
   omega.
   rewrite Zlength_get_buckets. assumption.
   apply Nat2Z.inj. rewrite <- Zlength_correct, <- Zlength_correct, Zlength_get_buckets. congruence.
@@ -265,55 +286,32 @@ Proof.
   unfold_data_at (data_at _ _ _ pm).
   rewrite field_at_data_at'. simpl nested_field_type. fold t_icell.
   pose (i := key mod N). fold i.
-  assert (h_i: 0 <= i < N). apply Z_mod_lt. unfold N. omega.
+  assert (h_i: 0 <= i < N). apply Z_mod_lt. rep_omega.
   rewrite wand_slice_array with (lo := i) (hi := i + 1).
   replace (i+1-i) with 1 by omega.
   rewrite sublist_len_1.
   erewrite data_at_singleton_array_eq by reflexivity.
-  forward_call (gv, Znth i (get_buckets m), key,  (field_address0 (tarray (tptr t_icell) 10) [ArraySubsc i]
+  forward_call (gv, get_bucket key m, key,  (field_address0 (tarray (tptr t_icell) N) [ArraySubsc i]
            (offset_val (nested_field_offset t_inthash [StructField _buckets]) pm)), Znth i buckets_p).
   entailer!.
   rewrite field_address0_offset. simpl nested_field_offset.
   rewrite Z.add_0_l. reflexivity.
   eapply field_compatible0_cons_Tarray. reflexivity. auto.
-  fold N. unfold i. unshelve epose proof (Z_mod_lt key N _). unfold N. omega. omega.
-  instantiate (Frame := [malloc_token Ews t_inthash pm; array_with_hole Ews (tptr t_icell) i (i + 1) 10 buckets_p pm;
+  unfold i. unshelve epose proof (Z_mod_lt key N _). rep_omega. rep_omega.
+  rewrite <- N_eq.
+  instantiate (Frame := [malloc_token Ews t_inthash pm; array_with_hole Ews (tptr t_icell) i (i + 1) N buckets_p pm;
   iter_sepcon (prod_curry icell_rep) (sublist 0 i (combine (get_buckets m) buckets_p));
   iter_sepcon (prod_curry icell_rep)
     (sublist (i + 1) N (combine (get_buckets m) buckets_p))]). unfold Frame. unfold fold_right_sepcon, i. entailer!.
-  split. assumption.
-  unfold get_buckets. rewrite Znth_map.
-  apply NoDupA_filter.
-  { intros x y ->. reflexivity. }
-  { rewrite Zlength_correct, seq_length. rep_omega. }
   Intros vret.
   destruct vret as [[p_ret r] tl]. unfold fst, snd in *.
   unfold icell_rep at 1; fold icell_rep. Intros q.
-  remember (match int_table.Raw.find (elt:=V) key (Znth i (get_buckets m)) with
-          | Some v0 => v0
-          | None => nullV
-          end) as old_v. destruct old_v as [old_v hold_v].
-  do 3 forward.
+  rewrite N_eq.
+  forward. entailer!. now destruct (maybe (int_table.find (elt:=V) key (get_bucket key m)) nullV).
+  do 2 forward.
   {
     entailer!.
-    {
-      case_eq (int_table.find (elt := V) key m).
-      + intros v0 hv0. apply int_table.find_2 in hv0.
-        rewrite get_buckets_spec' in hv0.
-        apply int_table.find_1 in hv0. unfold get_bucket, int_table.find, int_table.this in hv0.
-        fold i in hv0. rewrite hv0 in Heqold_v.
-        subst v0. reflexivity.
-      + intro hnone.
-        replace (int_table.Raw.find (elt := V) key (Znth i (get_buckets m)))
-                with (@None V) in Heqold_v.
-        now inversion Heqold_v.
-        symmetry. 
-        pose proof find_None as fn. unfold int_table.find in fn.
-        specialize (fn (get_bucket key m)). unfold get_bucket, int_table.this in fn. fold i in fn.
-        rewrite fn. intros v0 hcontr.
-        rewrite find_None in hnone. apply (hnone v0).
-        rewrite get_buckets_spec'. assumption.
-       }
+    { rewrite <- find_get_bucket. reflexivity. }
     
     allp_left v.
     sep_apply (wand_frame_elim' (data_at Ews (tptr t_icell) p_ret r * malloc_token Ews t_icell p_ret *
@@ -324,15 +322,15 @@ Proof.
     unfold inthash_rep.
     
     Exists (sublist 0 i buckets_p ++ pl :: sublist (i + 1) N buckets_p).
+    rewrite Zlength_app, Zlength_sublist, Zlength_cons, Zlength_sublist by rep_omega.
     rewrite focus_bucket with (key := key). fold i.
     
     unfold_data_at (data_at _ _ _ pm).
     rewrite field_at_data_at'. simpl nested_field_type.
-    rewrite wand_slice_array with (lo := i) (hi := i + 1).
+    rewrite <- N_eq, wand_slice_array with (lo := i) (hi := i + 1).
     replace (i+1-i) with 1 by omega.
     rewrite sublist_len_1.
     erewrite data_at_singleton_array_eq by reflexivity.
-
     
     do 2 replace (Znth i (sublist 0 i buckets_p ++ pl :: sublist (i + 1) N buckets_p))
     with pl.
@@ -349,40 +347,58 @@ Proof.
               (sublist (i + 1) N
              (combine (get_buckets m) buckets_p)).
     fold t_icell.
-    
-    replace (array_with_hole Ews (tptr t_icell) i (i + 1) 10
-          (sublist 0 i buckets_p ++ pl :: sublist (i + 1) N buckets_p)
-          (offset_val (nested_field_offset t_inthash [StructField _buckets]) pm)) with
-          (array_with_hole Ews (tptr t_icell) i (i + 1) 10 buckets_p pm).
+    simpl nested_field_offset. rewrite isptr_offset_val_zero.
 
-    replace (Znth i (get_buckets (int_table.add key v m))) with
-        (int_table.Raw.add key v (Znth i (get_buckets m))).
+    replace (array_with_hole Ews (tptr t_icell) i (i + 1) N
+          (sublist 0 i buckets_p ++ pl :: sublist (i + 1) N buckets_p) pm) with
+          (array_with_hole Ews (tptr t_icell) i (i + 1) N buckets_p pm).
+
+    replace (Znth i (get_buckets (int_table.add key v m))) with (int_table.Raw.add key v (Znth i (get_buckets m))).
     entailer!.
-    { autorewrite with sublist. omega. }
-    
     apply derives_refl.
     
-   
+    admit.
 
-    admit.
-    admit.
-    admit.
+    {
+      unfold array_with_hole.
+      rewrite sublist0_app1, sublist_sublist00.
+      rewrite sublist_app2, Zlength_sublist.
+      replace (i+1-(i-0)) with 1 by rep_omega.
+      rewrite sublist_1_cons, sublist_sublist, Z.add_0_l.
+      replace (N - (i - 0) - 1 + (i + 1)) with N by rep_omega.
+      simpl nested_field_offset. reflexivity.
+      auto.
+      omega. rep_omega. rep_omega. omega.
+      cbn. rep_omega. rewrite Zlength_sublist. rep_omega. rep_omega.
+      cbn. rep_omega. rep_omega. rewrite Zlength_sublist. rep_omega.
+      rep_omega. cbn. rep_omega.
+    }
+    
+    auto. admit.
     admit.
     
-    now autorewrite with sublist.
+    { rewrite app_Znth2, Zlength_sublist.
+      replace (i - (i -0)) with 0 by rep_omega.
+      reflexivity. 
+      omega. rep_omega. rewrite Zlength_sublist; rep_omega. }
+
     reflexivity.
-    now autorewrite with sublist.
-    autorewrite with sublist; omega.
-    omega.
-    fold N; omega.
-    fold N; autorewrite with sublist; omega.
+
+    { rewrite app_Znth2, Zlength_sublist.
+      replace (i - (i -0)) with 0 by rep_omega.
+      reflexivity. 
+      omega. rep_omega. rewrite Zlength_sublist; rep_omega. }
+
+    { rewrite Zlength_app, Zlength_sublist, Zlength_cons, Zlength_sublist; rep_omega. }
+    rep_omega. rep_omega.
+    autorewrite with sublist; rep_omega.
     autorewrite with sublist; omega.
  }
 
   cbn; omega.
   omega.
-  fold N; omega.
-  fold N; assumption.
+  rep_omega.
+  assumption.
   assumption.
 Admitted.
 
@@ -393,13 +409,13 @@ Proof.
   forward. 
   forward_loop
     (EX l1 l2: list (Z * V), EX r: val,
-      PROP ( l = l1 ++ l2; not (int_table.Raw.PX.In key l1) )
+      PROP ( {{ l }} = l1 ++ l2; not (int_table.Raw.PX.In key l1) )
      LOCAL (temp _r r; gvars gv; temp _r0 ppl; temp _key (Vint (Int.repr key)))
      SEP (mem_mgr gv;
           EX p: val, data_at Ews (tptr t_icell) p r * icell_rep l2 p;
           ALL l', (EX p, data_at Ews (tptr t_icell) p r * icell_rep l' p) -* EX pl: val, data_at Ews (tptr t_icell) pl ppl * icell_rep (l1 ++ l') pl)).
-  + Exists (@nil (Z*V)) l ppl pl.
-    entailer!. destruct H4 as [x hx]. inversion hx.
+  + Exists (@nil (Z*V)) {{ l }} ppl pl.
+    entailer!. destruct H3 as [x hx]. inversion hx.
     apply allp_right. intro.
     apply wand_refl_cancel_right.
   + Intros l1 l2 r p.
@@ -409,44 +425,37 @@ Proof.
     cbn. entailer!.
     Intro vret.
     do 2 forward.
-    replace l2 with (@nil (Z*V)) by intuition. rewrite app_nil_r.
-    replace (int_table.Raw.find (elt := V) key l1) with (@None V).
+    replace l2 with (@nil (Z*V)) in * by intuition.
+    rewrite app_nil_r in H0.
+    replace (maybe (int_table.find (elt:=V) key l) nullV) with nullV.        
     Exists vret r (@nil (Z*V)).
     unfold icell_rep at 2.
     entailer!.
     apply allp_right. intro v.
     sep_apply (allp_instantiate (fun l' =>
                                    (EX p0 : val, data_at Ews (tptr t_icell) p0 r * icell_rep l' p0) -*
-   (EX pl0 : val, data_at Ews (tptr t_icell) pl0 ppl * icell_rep (l1 ++ l') pl0)) [(key, v)]).
+   (EX pl0 : val, data_at Ews (tptr t_icell) pl0 ppl * icell_rep ({{l}} ++ l') pl0)) [(key, v)]).
     
     apply wand_derives. Exists vret. apply derives_refl.
     
-    replace (int_table.Raw.add key v l1) with (l1 ++ [(key, v)]).
+    replace (int_table.Raw.add key v {{ l }}) with ({{l}} ++ [(key, v)]).
     apply derives_refl.
     
-    { clear H0. induction l1 as [|[]]. reflexivity.
-      rewrite int_table.Raw.PX.In_alt in H2, IHl1.
-      cbn. rewrite if_false. rewrite IHl1. reflexivity.
-      intro hcontr. apply H2. 
+    { induction {{l}} as [|[]]. reflexivity.
+      rewrite int_table.Raw.add_equation, if_false, <- app_comm_cons, IHt.
+      reflexivity.
+      intro hcontr. apply H1. 
       destruct hcontr as [e he]. exists e. now apply SetoidList.InA_cons_tl.
-      intro heq. subst. apply H2. exists v0. constructor. constructor. }
-
-    case_eq (int_table.Raw.find (elt := V) key l1).
-    { intros v hv.
-      exfalso. apply H2. apply int_table.Raw.find_2 in hv.
-      rewrite int_table.Raw.PX.In_alt. exists v.
-      now apply int_table.Raw.PX.InA_eqke_eqk. }
-    easy.
+      intro heq. subst. apply H1. exists v0. constructor. now constructor. }
+    replace (int_table.find (elt := V) key l) with (@None V). reflexivity.
+    symmetry. rewrite find_None. intros v hv. apply H1. exists v. subst. apply hv.
   - destruct l2 as [|[k v]]. unfold icell_rep. Intros. contradiction.
     unfold icell_rep; fold icell_rep. Intros q.    
     forward. forward_if.
     ++ forward.
 
        Exists p r l2.
-       replace (match int_table.Raw.find (elt:=V) key (l1 ++ (key, v) :: l2) with
-           | Some v0 => v0
-           | None => nullV
-           end) with v.
+       replace (maybe (int_table.find (elt:=V) key l) nullV) with v.
        
        unfold icell_rep at 4; fold icell_rep. Exists q.
        entailer!.
@@ -456,10 +465,11 @@ Proof.
 
        apply wand_derives.
        Exists p. apply derives_refl.
-       replace (int_table.Raw.add key v' (l1 ++ (key, v) :: l2)) with (l1 ++ (key, v') :: l2).
+       replace (int_table.Raw.add key v' {{l}}) with (l1 ++ (key, v') :: l2).
        apply derives_refl.
 
-       { rename H2 into h.
+       { rewrite H0.
+         rename H1 into h.
          clear - h.
          induction l1 as [ | [k v'']].
          + cbn. now destruct Z_as_DT.eq_dec.
@@ -472,35 +482,56 @@ Proof.
            destruct hcontr as [e he]. exists e.
            apply SetoidList.InA_cons_tl. assumption. }
        
-       { replace (int_table.Raw.find (elt := V) key (l1 ++ (key, v) :: l2)) with (Some v). reflexivity.
-         symmetry. apply int_table.Raw.find_1. assumption.
-         unfold int_table.Raw.PX.MapsTo.
-         rewrite SetoidList.InA_app_iff. right. constructor. easy.
+       { replace (int_table.find (elt := V) key l) with (Some v). reflexivity.
+         symmetry. apply int_table.find_1. 
+         unfold int_table.MapsTo, int_table.Raw.PX.MapsTo.
+         rewrite H0, SetoidList.InA_app_iff. right. constructor. easy. }
+    ++ forward. simpl offset_val.
+       Exists (l1 ++ [(k,v)]) l2 (offset_val 8 p) q.
+       entailer!.
+       split.
+       { rewrite <- app_assoc. easy. }
+       { intros [e hcontr%SetoidList.InA_app].
+         destruct hcontr.
+         + apply H1. exists e. assumption.
+         + apply SetoidList.InA_singleton in H12.
+           compute in H12. omega. }
+       
+       unfold_data_at (data_at _ _ _ p).
+       rewrite (field_at_data_at' _ _ [StructField _next]). simpl nested_field_type. simpl nested_field_offset.
+       entailer!.
+
+       apply allp_right. intro l'.
+       allp_left ((k,v)::l').
+       rewrite <- wand_sepcon_adjoint.
+       sep_apply (wand_frame_elim' ((data_at Ews (tptr t_icell) p r *
+   (malloc_token Ews t_icell p *
+    (field_at Ews t_icell [StructField _key] (Vint (Int.repr k)) p *
+     field_at Ews t_icell [StructField _value] (V_repr v) p))) *
+  (EX p0 : reptype (tptr t_icell), data_at Ews (tptr t_icell) p0 (offset_val 8 p) * icell_rep l' p0))).
+       cbn. Intro p0.
+       Exists p p0. unfold_data_at (data_at _ _ _ p).
+       rewrite (field_at_data_at _ _ [StructField _next]), field_address_offset.
+       entailer!.
+       auto with field_compatible.
+       rewrite <- app_assoc. apply derives_refl.
 Qed.
+
 
 Lemma body_inthash_lookup: semax_body Vprog Gprog f_inthash_lookup inthash_lookup_spec.
 Proof.
   start_function.
   unfold inthash_rep.
   Intros buckets_p.
-  remember (combine (get_buckets m) buckets_p) as l.
-  remember (key mod N) as i.
-  remember (iter_sepcon (prod_curry icell_rep) l) as buckets_rep eqn:hb.
-  pose proof hb as save_buckets_rep.
-  replace l with (sublist 0 i l ++ [(Znth i (get_buckets m), Znth i buckets_p)]
-                          ++ sublist (i+1) (Zlength l) l) in hb.
-  do 2 rewrite iter_sepcon_app in hb.
-  simpl iter_sepcon in hb.
-  subst buckets_rep.
-  Intros.
+  rewrite focus_bucket with (key := key) by assumption. Intros.
   forward.
-  { pose proof (Z_mod_lt key 10).
+  { pose proof (Z_mod_lt key N).
     entailer. }
   { 
-    change 10 with N.
-    rewrite <- Heqi.
+    remember (key mod N) as i.
     remember (Znth i buckets_p) as q0.
     remember (Znth i (get_buckets m)) as kvs.
+    remember (combine (get_buckets m) buckets_p) as l.
     forward_while (
         EX kvs1 kvs2: list (Z * V), EX q: val,
      PROP ( kvs = kvs1 ++ kvs2 /\ not (int_table.Raw.PX.In key kvs1))
@@ -509,12 +540,15 @@ Proof.
      iter_sepcon (prod_curry icell_rep) (sublist 0 i l);
      icell_rep kvs2 q;
      icell_rep kvs2 q -* icell_rep kvs q0;
-     emp; iter_sepcon (prod_curry icell_rep) (sublist (i + 1) (Zlength l) l)))%assert.
+     emp; iter_sepcon (prod_curry icell_rep) (sublist (i + 1) N l)))%assert.
     + Exists (@nil (Z*V)) kvs q0.
       entailer!.
-      { rewrite int_table.Raw.PX.In_alt in H5. destruct H5 as [e he].
-        inv he. }      
+      { rewrite int_table.Raw.PX.In_alt in H6. destruct H6 as [e he].
+        inv he. }
+      replace (Zlength (combine (get_buckets m) buckets_p)) with N. cancel.
       apply wand_refl_cancel_right.
+      rewrite Zlength_combine, Z.min_l, Zlength_get_buckets. reflexivity.
+      rewrite Zlength_get_buckets; omega.
     + entailer!.
     + destruct kvs2. assert_PROP (q = nullval). entailer!. intuition.
       subst q. contradiction.
@@ -529,10 +563,12 @@ Proof.
         replace (int_table.find key m) with (Some v_sig).
         entailer!.
         unfold inthash_rep. Exists buckets_p.
-        rewrite <- save_buckets_rep.
+        rewrite focus_bucket with (key := key) by rep_omega.
         entailer!.
-        eapply modus_ponens_wand'. unfold icell_rep at 2; fold icell_rep.
-        Exists q1. entailer. 
+        sep_apply (wand_frame_elim'
+                     (malloc_token Ews t_icell q * data_at Ews t_icell (vint key, (V_repr (exist is_pointer_or_null v hv), q1)) q * icell_rep kvs2 q1)).
+        unfold icell_rep at 2; fold icell_rep.
+        Exists q1. entailer. apply derives_refl.
         symmetry. eapply int_table.find_1. rewrite get_buckets_spec.
         rewrite (proj1 H1), SetoidList.InA_app_iff. right. constructor. reflexivity.
       - forward. Exists (kvs1 ++ [(k,v)], kvs2, q1).
@@ -553,39 +589,14 @@ Proof.
       + forward.
         replace (int_table.find (elt := V) key m) with (@None V).
         unfold inthash_rep. Exists buckets_p.
-        rewrite <- save_buckets_rep. entailer!. apply modus_ponens_wand.
-        replace kvs2 with (@nil (Z*V)) in H1 by intuition.
-        rewrite app_nil_r in H1.
-        remember (int_table.find (elt := V) key m) as f. destruct f.
-        symmetry in Heqf. apply int_table.find_2 in Heqf.
-        rewrite get_buckets_spec in Heqf.
-        destruct H1 as [hnth hnin].
-        rewrite hnth in Heqf.
-        exfalso. apply hnin.
-        rewrite int_table.Raw.PX.In_alt.
-        exists v. apply int_table.Raw.PX.InA_eqke_eqk. assumption.
-        reflexivity.
+        rewrite focus_bucket with (key := key). entailer!. apply modus_ponens_wand.
+        assumption.
+        replace kvs2 with (@nil (Z*V)) in H1 by intuition. rewrite app_nil_r in H1.
+        symmetry. apply find_None.
+        intros v hv. apply (proj2 H1). exists v.
+        rewrite <- (proj1 H1). rewrite get_buckets_spec' in hv.
+        unfold int_table.MapsTo in hv. apply hv.
   }
-  assert (hlenl: Zlength l = N).
-  { subst l. rewrite Zlength_correct, combine_length, Min.min_l, <- Zlength_correct, Zlength_get_buckets.
-    reflexivity.
-     apply Nat2Z.inj_le. rewrite <- Zlength_correct, <- Zlength_correct, H0, Zlength_get_buckets. omega. }
-  { symmetry.
-  rewrite <- (sublist_same_gen 0 (Zlength l) l) at 1 by omega. rewrite hlenl.
-  assert (0 <= i < 10). subst i. apply Z_mod_lt. computable.
-  assert (N = 10) by reflexivity. 
-  erewrite sublist_split. f_equal.
-  erewrite sublist_split. f_equal.
-  rewrite sublist_len_1. subst l. rewrite <- nth_Znth, <- nth_Znth, <- nth_Znth, combine_nth.
-  reflexivity.
-  apply Nat2Z.inj.
-  now rewrite <- Zlength_correct, <- Zlength_correct, Zlength_get_buckets.
-  rep_omega.
-  rewrite Zlength_get_buckets. omega.
-  rewrite Zlength_correct, combine_length. split. easy.
-  rewrite Min.min_r. rewrite <- Zlength_correct. omega. 
-  apply Nat2Z.inj_le. rewrite <- Zlength_correct, <- Zlength_correct, H0, Zlength_get_buckets. omega.
-  omega.  omega. omega. omega. omega. }
 Qed.
 
 Lemma body_inthash_new: semax_body Vprog Gprog f_inthash_new inthash_new_spec.
@@ -607,31 +618,30 @@ Proof.
        LOCAL (temp _p vret; gvars gv)
        SEP (mem_mgr gv;
               malloc_token Ews t_inthash vret;
-              data_at Ews t_inthash (list_repeat (Z.to_nat i) nullval ++ list_repeat (Z.to_nat (N-i)) Vundef) vret))%assert.
-    + unfold N. omega.
-    + now compute.
-    + entailer!. unfold N. omega.
-      rewrite Z2Nat.inj_0. unfold list_repeat at 1.
-      rewrite app_nil_l. apply derives_refl.
+              data_at Ews t_inthash (Zrepeat i nullval ++ Zrepeat (N-i) Vundef) vret))%assert.
+    + entailer!. apply data_at__data_at. reflexivity.
     + forward.
       entailer!.
       autorewrite with sublist.
-      rewrite upd_Znth0, semax_lemmas.cons_app.
-      rewrite <- list_repeat_app', <- app_assoc.
-      autorewrite with sublist.
-      change (list_repeat (Z.to_nat 1) nullval) with [Vint (Int.repr 0)].
-      replace (N-(i+1)) with (N-i-1) by omega.
-      apply derives_refl. omega. omega.
-    + change (list_repeat (Z.to_nat (N - N)) Vundef) with (@nil val).
-      rewrite app_nil_r.
-      forward. Exists vret. unfold inthash_rep, int_table.empty.
-      Exists (list_repeat (Z.to_nat N) nullval).
+      rewrite Zlength_Zrepeat, Z.sub_diag, upd_Znth0, Zlength_Zrepeat by rep_omega.
+      replace (Zrepeat (N - i) Vundef) with (Vundef :: Zrepeat (N - (i + 1)) Vundef).
+      rewrite sublist_1_cons.
+      unfold Zrepeat. rewrite Z2Nat.inj_add, repeat_plus, sublist_repeat by omega.
+      change (Z.to_nat 1) with 1%nat.
+      cbn. replace (N - i - 1 - 0) with (N - (i+1)) by omega.
+      rewrite <- app_assoc.
+      apply derives_refl.
+      change (Vundef :: Zrepeat (N - (i + 1)) Vundef) with (Zrepeat 1 Vundef ++ Zrepeat (N-(i+1)) Vundef).
+      unfold Zrepeat. rewrite <- repeat_plus. rewrite <- Z2Nat.inj_add by omega.
+      replace  (1 + (N - (i + 1))) with (N - i) by omega. reflexivity.
+    + forward. Exists vret. unfold inthash_rep, int_table.empty.
+      Exists (Zrepeat N nullval).
       rewrite iter_sepcon_emp'.
       entailer!.
       { intros [l p] hxl. pose proof hxl as hxr.
         apply in_combine_l in hxl. apply in_combine_r in hxr.
         cbn in hxl.
-        apply list_in_map_inv in hxl. apply in_list_repeat in hxr.
+        apply list_in_map_inv in hxl. rewrite <- Zrepeat_fold in hxr. apply in_list_repeat in hxr.
         destruct hxl as [? []].
         subst. cbn.
         apply pred_ext; entailer. }}
